looping arm example

Completeness.v
@@ -77,4 +77,117 @@ Section BudgetTotalIsNecessary.
 
 End BudgetTotalIsNecessary.
 
+Section LoopingArmUnderCase.
+  Variables (Φ : path_condition) (σ : valuation) (S : symvars).
+  Variables (x : var) (l' : lit).
+
+  Hypothesis HmodPhi : σ ⊨ Φ.
+  Hypothesis Hsx     : S x = true.
+  Hypothesis Hmodx   : σ ⊨ PCVar x.
+  Hypothesis Hsf     : S self_app_var = false.
+
+  Definition case_alts : list alt :=
+    Alt "T" [] (ELit l') :: Alt "F" [] self_app :: nil.
+  Definition case_sym : expr := ECase (EIf (EVar x) (ECon "T") (ECon "F")) case_alts.
+  Definition case_con : expr := ECase (ECon "T") case_alts.
+
+  Lemma case_guard_cond : models_cond σ S (EVar x).
+  Proof.
+    exists (PCVar x). split; [| exact Hmodx].
+    intros Γ Hfree. simpl. rewrite (Hfree x Hsx). reflexivity.
+  Qed.
+
+  Lemma case_alts_contains : Forall2 (contains_alt σ S) case_alts case_alts.
+  Proof.
+    apply Forall2_cons; [| apply Forall2_cons; [| apply Forall2_nil]].
+    - apply Cont_Alt; [apply Forall_nil | apply Cont_Lit].
+    - apply Cont_Alt; [apply Forall_nil |].
+      unfold self_app, self_app_fun, self_app_body.
+      apply Cont_App; (apply Cont_Lam; [exact Hsf |]);
+        (apply Cont_App; apply Cont_Var_Bound; exact Hsf).
+  Qed.
+
+  Lemma case_contains : contains σ S case_sym case_con.
+  Proof.
+    apply Cont_Case; [| exact case_alts_contains].
+    apply Cont_If_True; [exact case_guard_cond | apply Cont_Con].
+  Qed.
+
+  Lemma case_con_concore : concore_expr case_con.
+  Proof.
+    apply Con_Case; [apply Con_Con |].
+    apply Forall_cons; [| apply Forall_cons; [| apply Forall_nil]].
+    - apply Con_Alt. apply Con_Lit.
+    - apply Con_Alt. unfold self_app, self_app_fun, self_app_body.
+      apply Con_App; apply Con_Lam; apply Con_App; apply Con_Var.
+  Qed.
+
+  Lemma case_con_converges : Φ ; · ⊢ case_con ⇓ (ELit l').
+  Proof.
+    unfold case_con.
+    eapply Eval_Case.
+    - eapply Eval_Con. reflexivity.
+    - simpl. eapply FoldAlts_Con.
+      + reflexivity.
+      + simpl. destruct (string_dec "T" "T"); [reflexivity | congruence].
+      + simpl. apply Eval_Lit.
+  Qed.
+
+  Lemma case_budget_total : budget_total Φ · case_sym.
+  Proof.
+    exists 3%nat. intros n Hn. destruct n as [| [| [| m]]]; [lia | lia | lia |].
+    destruct (self_app_has_value_at_every_budget (Datatypes.S (Datatypes.S m))
+                (Φ ∧ ¬ PCVar x) ·) as [vf Hvf].
+    exists (EIf (EVar x) (ELit l') vf).
+    unfold case_sym.
+    eapply Eval_Case.
+    - eapply Eval_If with (pc_c := PCVar x).
+      + apply Eval_SymVar. reflexivity.
+      + reflexivity.
+      + eapply Eval_Con. reflexivity.
+      + eapply Eval_Con. reflexivity.
+    - simpl. eapply FoldAlts_If.
+      + reflexivity.
+      + simpl. eapply FoldAlts_Con.
+        * reflexivity.
+        * simpl. destruct (string_dec "T" "T"); [reflexivity | congruence].
+        * simpl. apply Eval_Lit.
+      + simpl. eapply FoldAlts_Con.
+        * reflexivity.
+        * simpl. destruct (string_dec "F" "T"); [congruence |].
+          simpl. destruct (string_dec "F" "F"); [reflexivity | congruence].
+        * simpl. exact Hvf.
+  Qed.
+
+  Theorem case_target_conclusion :
+    exists h, forall n, (h <= n)%nat ->
+      exists v_sym, eval (Fin n) Φ · case_sym v_sym /\ contains σ S v_sym (ELit l').
+  Proof.
+    exists 3%nat. intros n Hn. destruct n as [| [| [| m]]]; [lia | lia | lia |].
+    destruct (self_app_has_value_at_every_budget (Datatypes.S (Datatypes.S m))
+                (Φ ∧ ¬ PCVar x) ·) as [vf Hvf].
+    exists (EIf (EVar x) (ELit l') vf). split.
+    - unfold case_sym.
+      eapply Eval_Case.
+      + eapply Eval_If with (pc_c := PCVar x).
+        * apply Eval_SymVar. reflexivity.
+        * reflexivity.
+        * eapply Eval_Con. reflexivity.
+        * eapply Eval_Con. reflexivity.
+      + simpl. eapply FoldAlts_If.
+        * reflexivity.
+        * simpl. eapply FoldAlts_Con.
+          -- reflexivity.
+          -- simpl. destruct (string_dec "T" "T"); [reflexivity | congruence].
+          -- simpl. apply Eval_Lit.
+        * simpl. eapply FoldAlts_Con.
+          -- reflexivity.
+          -- simpl. destruct (string_dec "F" "T"); [congruence |].
+             simpl. destruct (string_dec "F" "F"); [reflexivity | congruence].
+          -- simpl. exact Hvf.
+    - apply Cont_If_True; [exact case_guard_cond | apply Cont_Lit].
+  Qed.
+
+End LoopingArmUnderCase.
+
 End Completeness.
